
\documentclass[../Main/main]{subfiles}


\begin{document}

\renewcommand{\blockName}{ Martin Azpillaga }
\unit{ $ 2nd laboratory $ }
{
	\proposition{ $ Power series $ }
	{
		\study
		{
			\summation{ n(n+1)z^n }{ n }[ 1 ]
		}
		\demonstration
		{
			\step{ $Naming$ }
			{
				R $ radius of convergence of the series $.
				\all{ n \in \N }
				{
					\be{ c_n }{ n(n+1) }
				}
			}.

			\step{ $Convergence domain$ }
			{
				\limit{ \frac{ c_n }{ c_{n+1} } }{ n } = \limit{ \frac{ n(n+1) }{ (n+1)(n+1) } }{ n } = 1.

				$Quotient test:$.
				R^{-1} = \superiorlimit{ |c_n|^{\frac{ 1 }{ n }} }{ n } = 1 \imp R = 1.

				$Cauchy-Hadamard theorem:$.

				\summation{ n(n+1)z^n }{ n }[ 1 ] $ convergent over $ \D.
				\summation{ n(n+1)z^n }{ n }[ 1 ] $ divergent  over $ \C \setminus \closed{\D}.
				\all{ K \subset \D }[ K $ compact $ ]
				{
					\summation{ n(n+1)z^n }{ n }[ 1 ] $ uniformly convergent over $  K
				}.

				$ Define $.

				\definedFunction{ f }{ \D }{ \C }{ z }{ z \summation{ n(n+1)z^{n-1} }{ n }[ 1 ] }
			}.


			\step{ $Sum$ }
			{
				\definedFunction{ g }{ \D }{ \C }{ z }{ \summation{ n(n+1)z^{n-1} }{ n }[ 1 ] }.

				$UCI theorem:$.

				\integral{ g(t) }{ dt }{ 0 }[ z ] = \summation{ (n+1)z^n }{ n }[ 1 ].
				\definedFunction{ h }{ \D }{ \C }{ z }{ \summation{ (n+1)z^n }{ n }[ 1 ] }.
				\integral{ h(t) }{ dt }{ 0 }[ z ] =  \summation{ z^{n+1} }{ n }[ 1 ] = \summation{ z^n }{ n }[ 0 ] = \frac{ 1 }{ 1-z }.

				h(z) = \partialderivative{ \frac{ 1 }{ 1-z } }{ z } = \frac{ 1 }{ (1-z)^2 }.
				g(z) = \partialderivative{ h(z) }{ z } = \frac{ 2 }{ (1-z)^3 }.

				f(z) = \frac{ 2z }{ (1-z)^3 }
			}.


			\step{ $Application$ }
			{
				$In particular:$.

				\summation{ (-1)^n \frac{ n(n+1) }{ 2^n } }{ n }[ 1 ] = f(-\frac{ 1 }{ 2 } ) = \frac{ -2^3 }{ 3^3 }
			}
		}
	}
	
}



\end{document}