



\documentclass[../Main/main]{subfiles}


\begin{document}


\unit{ $ New $ }
{

	
	\proposition{ $ Power series theorem $ }
	{
		\letbe
		{
			
		}
		\holds
		{
			Part II,III,IV
		}
		\demonstration
		{
			$ Follow 3 steps $.
			
			\steps{ 1 }{ Uniform convergence in compacts of $D(a,R)$ }
			{
				\definedFunction{ g_n }{ \C }{ \C }{ z }{ c_n(z-a)^n }.
				\all{ \rho \in \R }[ \rho < R ]
				{
					\all{ z \in \closed{D(a,\rho)} }
					{
						|g_n(z)| = |c_n||z-a|^n \leq |c_n|\rho^n
					}.

					\be{ M_n }{ |c_n|\rho^n }.

					\limit{ (|c_n|\rho^n)^{1/n} }{ n } = \rho \limit{ |c_n|^{1/n} }{ n } = \frac{ \rho }{ R } < 1.

					$Root test$ \imp \summation{ M_n }{ n }[ 0 ] $ convergent $.

					$M-Weierstrass$ \imp \summation{ c_n(z-a)^n }{ n }[ 0 ] $ uniformly convergent over compacts of $ D(a,\rho)
				}.

				\summation{ c_n(z-a)^n }{ n }[ 0 ] $ uniformly convergent over compacts of $ D(a,r).

				\be{ f(z) }{ \summation{ g_n(z) }{ n }[ 0 ] }.

				g $ uniformly convergent $ \imp f $ continuous $
			}.
			
			\steps{ 2 }{ IV. R' }
			{
				\be{ \tilde{f}(z) }{ \summation{ nc_n(z-a)^{n-1} }{ n }[ 1 ] }.

				\tilde{f}(z) = \summation{ (n+1)c_{n+1}(z-a)^n }{ n }[ 0 ].

				\frac{ 1 }{ R' } = \limit{ (n+1)|c_{n+1}|^{1/n} }{ n } = \limit{ (n+1)^{1/n}|c_{n+1}|^{1/n} }{ n } = \limit{ (|c_{n+1}|^{1/n+1})^{\frac{ n+1 }{ n }} }{ n } = \frac{ 1 }{ R }.

				R' = R

			}

			\steps{ 3 }{ III }
			{
				\tilde{f} $well defined in $ D(a,R).
				\all{ z_0 \in D(a,R) }
				{
					
						\abs{ \frac{ f(z) - f(z_0) }{ z - z_0 } - \tilde{f}(z_0)} \convergesto 0?.

						\all{ n \in \N }
						{
							\be{ S_n(z) }{ \summation{ f_k(z) }{ k }[ 0 ][ n ] }.
							\be{ R_n(z) }{ \summation{ f_k(z) }{ k }[ n+1 ] }.
							f(z) = S_n(z) + R_n(z).

							\tilde{f}(z) = \tilde{S_n}(z) + \tilde{R_n}(z).

							R_n(z), \tilde{R_n}(z) \convergesto 0

						}.


						\all{ \epsilon \in \R^+ }
						{
							\abs{ \frac{ f(z) - f(z_0) }{ z - z_0 } } = \abs{ \frac{ S_n(z) - S_n(z_0) }{ z - z_0 } + \frac{ R_n(z) - R_n(z_0) }{ z - z_0 } - \tilde{S_n}(z_0) - \tilde{R_n}(z_0) }.

							\all{ \rho \in \R }[ |z_0 - a| < \rho < R ]
							{
								\abs{ \tilde{R_n}(z_0) } \leq \summation{ k|c_k|\rho^{k-1} }{ k }[ n+1 ] < \frac{ \epsilon }{ 3 } ( n \geq n_1 ).
							}.

							\abs{ \frac{ R_n(z) - R_n(z_0) }{ z - z_0 } } \leq \summation{ |c_k||\frac{ (z-a)^k - (z_0 - a)^k }{ z - z_0 }| }{ k }[ n+1 ].

							\frac{ a^k - b^k }{ a-b } = a^{k-1} - a^{k-2}b + --- + b^{k-1}.

							\leq \summation{ |c_k|(|z-a|^{k-1} + |z-a|^{k-2}|z_0-a| + --- + |z_0 -a|^{k-1} }{ k }[ n+1 ].

							|z-a|, |z_0| < \rho.

							\leq \summation{ |c_k|k\rho^{k-1} }{ k }[ n+1 ] < \frac{ \epsilon }{ 3 } ( n \geq n_1 ).

							\abs{ \frac{ S_n(z) - S_n(z_0) }{ z - z_0 } - \tilde{S_n}(z_0) } < \frac{ \epsilon }{ 3 } ( S_n' = \tilde{S_n} ) ( n \geq n_2 ).

							\all{ n \in \N }[ n \geq \max( n_1, n_2 )  ]
							{
								\abs{ \frac{ f(z) - f(z_0) }{ z - z_0 } } < \epsilon
							}
						}		
				}
			}
		}
	}
	
	
			
	\proposition{ $ functions associated to series are $ \Cc^{\infty} }
	{
		\letbe
		{
			f(z) = \sum{ c_n(z-a)^n }{ n }[ 0 ] $ series $.
			R $ radius of convergence of $ f
		}
		\holds
		{
			f \in \Cc^{\infty} $ over $ D(a,R).
			\all{ n \in \N }
			{
				f^{n)} \in \Hc(D(a,R))
			}.

			c_k = \frac{ f^{k)} }{ k! }.

			$ series associated to $ f $ is unique $
		}
		\demonstration
		{
			f^{k)}(z) = \sum{ n(n-1)---(n-k+1)c_n(z-a)^{n-k} }{ n }[ k ].

			f^{k)}(a) = k! c_k.

			c_k = \frac{ f^{k)}(a) }{ k! }
		}
	}
	
	
	\example{ $ Geometric series $ }
	{
		\letbe
		{
			a \as 0.
			c_n : 0
		}
		\is{ \sum{ z^n }{ n }[ 0 ] }{ $ convergent in $ \D }
		{
			R = \frac{ c_n }{ c_{n+1} } = 1
		}
		\holds
		{
			\sum{ z^n }{ n }[ 0 ] = \frac{ 1 }{ 1-z }.
			\sum{ nz^{n-1} }{ n }[ 0 ] = \frac{ 1 }{ (1-z)^2 }.
			\sum{ \frac{ z^{n+1} }{ n+1 } }{ n }[ 0 ] = - \log( 1-z )
		}
		\demonstration
		{
			\all{ z \in \D }
			{
				\sum{ z^n }{ n }[ 0 ] $ geometric series $.
				\sum{ z^n }{ n }[ 0 ] = \frac{ 1 }{ 1-z }
			}.

			II $ differentiating $.

			III $ integrating $
		}
	}
	
	
	\example{ $ Series not centered in 0 $ }
	{
		\letbe
		{
			a \as i.
			c_n \as \frac{ n+1 }{ 5^{n+1} }
		}
		\is{ item }{ $ a/an entity $ }
		{
			\sum{ \frac{ n(z-i)^{n-1} }{ 5^n } }{ n }[ 1 ].

			 = \frac{ 1 }{ 5 } \sum{ n \frac{ z-i }{ 5 }^{n-1} }{ n }[ 1 ] = \frac{ 1 }{ 5 } \sum{ nu^{n-1} }{ n }[ 1 ].

			 S(u) = \tilde{S'}(u).

			 \tilde{S}(u) = \frac{ 1 }{ 5 } \sum{ u^n }{ n }[ 1 ] = \frac{ u }{ 5(1-u) }.

			 S(u) = \frac{ 1 }{ 5(1-u)^2 }.

			 S(z) = \frac{ 5 }{ (5+i-z)^2 } $ over $ D(i,5).


		}
	}
	
	
	\example{ $ Radius of convergence without quotient test $ }
	{
		\letbe
		{
			\sum{ \frac{ (-1)^n }{ n(n+1) }(z-2)^{n(n+1)} }{ n }[ 1 ]
		}
		\is{ R }{ $ a/an entity $ }
		{
			\limit{ c_n }{ c_{n+1} } \nexists.

			\limit{ \frac{ 1 }{ n(n+1) }^{\frac{ 1 }{ n(n+1) }} }{ n } = 1.

			$ ignore zeros $.
		}
	}
	
	
	
	



}


\end{document}